Impl/FlushPolicyImpl.i.dfy
@@ -31,6 +31,10 @@ module FlushPolicyImpl {
   import opened BucketsLib
   import opened BucketWeights
 
+  import opened InterpretationDiskOps
+  import opened ViewOp
+  import opened DiskOpModel
+
   // temporarily moving method to cache
   // method biggestSlot(shared buckets: lseq<MutBucket>) returns (res : (uint64, uint64))
   // requires MutBucket.InvLseq(buckets)
@@ -61,9 +65,9 @@ module FlushPolicyImpl {
     slots: seq<uint64>, i: uint64)
   returns (action : FlushPolicyModel.Action)
   requires 0 <= i as int < |stack|
-  requires s.Inv()
-  requires FlushPolicyModel.ValidStackSlots(s.I(), stack, slots)
-  ensures action == FlushPolicyModel.getActionToSplit(s.I(), stack, slots, i)
+  requires s.BCInv()
+  requires FlushPolicyModel.ValidStackSlots(s.IBlockCache(), stack, slots)
+  ensures action == FlushPolicyModel.getActionToSplit(s.IBlockCache(), stack, slots, i)
   {
     FlushPolicyModel.reveal_getActionToSplit();
 
@@ -96,12 +100,12 @@ module FlushPolicyImpl {
   method getActionToFlush(linear inout s: ImplVariables, stack: seq<BT.G.Reference>, slots: seq<uint64>)
   returns (action : FlushPolicyModel.Action)
   requires |stack| <= 40
-  requires old_s.Inv()
-  requires FlushPolicyModel.ValidStackSlots(old_s.I(), stack, slots)
+  requires old_s.BCInv()
+  requires FlushPolicyModel.ValidStackSlots(old_s.IBlockCache(), stack, slots)
   decreases 0x1_0000_0000_0000_0000 - |stack|
-  ensures s.W()
+  ensures s.BCInv()
   ensures s.Ready?
-  ensures (s.I(), action) == FlushPolicyModel.getActionToFlush(old_s.I(), stack, slots)
+  ensures (s.IBlockCache(), action) == FlushPolicyModel.getActionToFlush(old_s.IBlockCache(), stack, slots)
   {
     FlushPolicyModel.reveal_getActionToFlush();
 
@@ -149,23 +153,22 @@ module FlushPolicyImpl {
   }
 
   method runFlushPolicy(linear inout s: ImplVariables, io: DiskIOHandler)
-  requires old_s.Inv()
+  requires old_s.BCInv() && old_s.Ready?
   requires io.initialized()
-  requires old_s.Ready?
   requires BT.G.Root() in old_s.cache.I()
   requires |old_s.ephemeralIndirectionTable.I().graph| <= IT.MaxSize() - 3
   modifies io
-  ensures s.W()
-  ensures s.Ready?
-  ensures FlushPolicyModel.runFlushPolicy(old_s.I(), old(IIO(io)), s.I(), IIO(io))
-  {
-    FlushPolicyModel.reveal_runFlushPolicy();
+  ensures s.W() && s.Ready?
 
+  ensures ValidDiskOp(diskOp(IIO(io)))
+  ensures IDiskOp(diskOp(IIO(io))).jdop.NoDiskOp?
+  ensures IOModel.betree_next_dop(old_s.IBlockCache(), s.IBlockCache(),
+      IDiskOp(diskOp(IIO(io))).bdop)
+  {
     LruModel.LruUse(s.lru.Queue(), BT.G.Root());
     inout s.lru.Use(BT.G.Root());
-    assert SBCM.IBlockCache(s.I()) == SBCM.IBlockCache(old_s.I());
 
-    FlushPolicyModel.getActionToFlushValidAction(s.I(), [BT.G.Root()], []);
+    FlushPolicyModel.getActionToFlushValidAction(s.IBlockCache(), [BT.G.Root()], []);
     var action := getActionToFlush(inout s, [BT.G.Root()], []);
 
     match action {
@@ -174,23 +177,28 @@ module FlushPolicyImpl {
       }
       case ActionSplit(parentref, slot) => {
         var _, parent_children := s.cache.GetNodeInfo(parentref);
+        SplitModel.doSplitCorrect(s.IBlockCache(), parentref, parent_children.value[slot], slot as int);
         doSplit(inout s, parentref, parent_children.value[slot], slot);
       }
       case ActionRepivot(ref) => {
+        LeafModel.repivotLeafCorrect(s.IBlockCache(), ref, s.cache.I()[ref]);
         repivotLeaf(inout s, ref);
       }
       case ActionFlush(parentref, slot) => {
         var _, parent_children := s.cache.GetNodeInfo(parentref);
         var childref := parent_children.value[slot];
+        FlushModel.flushCorrect(s.IBlockCache(), parentref, slot as int, childref,s.cache.I()[childref]);
         flush(inout s, parentref, slot, childref);
       }
       case ActionGrow => {
+        GrowModel.growCorrect(s.IBlockCache());
         grow(inout s);
       }
       case ActionEvict => {
         EvictOrDealloc(inout s, io);
       }
       case ActionFail => {
+        assert IOModel.noop(old_s.IBlockCache(), s.IBlockCache());
         print "ActionFail\n";
       }
     }
